src/lowparse/LowParse.SteelST.List.Iterator.fsti
@@ -7,6 +7,34 @@ module AP = LowParse.SteelST.ArrayPtr
 module SZ = FStar.SizeT
 module R = Steel.ST.Reference
 
+val list_iterator_strong
+  (#k: parser_kind)
+  (#t: Type0) // gen_elim universe issue
+  (p: parser k t)
+  (va0: v parse_list_kind (list t))
+  (a0: byte_array)
+  (l: list t) // the list of already processed elements
+  (va: v parse_list_kind (list t))
+: Tot vprop
+
+val list_iterator_strong_facts
+  (#opened: _)
+  (#k: parser_kind)
+  (#t: Type)
+  (p: parser k t)
+  (va0: v parse_list_kind (list t))
+  (a0: byte_array)
+  (l: list t)
+  (va: v parse_list_kind (list t))
+: STGhost unit opened
+    (list_iterator_strong p va0 a0 l va)
+    (fun _ -> list_iterator_strong p va0 a0 l va)
+    True
+    (fun _ ->
+      k.parser_kind_subkind == Some ParserStrong /\
+      va0.contents == l `List.Tot.append` va.contents
+    )
+
 val list_iterator
   (#k: parser_kind)
   (#t: Type0) // gen_elim universe issue
@@ -16,7 +44,32 @@ val list_iterator
   (va: v parse_list_kind (list t))
 : Tot vprop
 
-val list_iterator_parser_kind
+val list_iterator_of_list_iterator_strong
+  (#opened: _)
+  (#k: parser_kind)
+  (#t: Type0) // gen_elim universe issue
+  (p: parser k t)
+  (va0: v parse_list_kind (list t))
+  (a0: byte_array)
+  (l: list t)
+  (va: v parse_list_kind (list t))
+: STGhostT unit opened
+    (list_iterator_strong p va0 a0 l va)
+    (fun _ -> list_iterator p va0 a0 va)
+
+val list_iterator_strong_of_list_iterator
+  (#opened: _)
+  (#k: parser_kind)
+  (#t: Type0) // gen_elim universe issue
+  (p: parser k t)
+  (va0: v parse_list_kind (list t))
+  (a0: byte_array)
+  (va: v parse_list_kind (list t))
+: STGhostT (Ghost.erased (list t)) opened
+    (list_iterator p va0 a0 va)
+    (fun l -> list_iterator_strong p va0 a0 l va)
+
+let list_iterator_parser_kind
   (#opened: _)
   (#k: parser_kind)
   (#t: Type)
@@ -31,8 +84,27 @@ val list_iterator_parser_kind
     (fun _ ->
       k.parser_kind_subkind == Some ParserStrong
     )
+= let _ = list_iterator_strong_of_list_iterator _ _ _ _ in
+  list_iterator_strong_facts _ _ _ _ _;
+  list_iterator_of_list_iterator_strong _ _ _ _ _
 
-val list_iterator_begin
+val list_iterator_strong_begin
+  (#opened: _)
+  (#k: parser_kind)
+  (#t: Type)
+  (p: parser k t)
+  (#va0: v parse_list_kind (list t))
+  (a0: byte_array)
+: STGhost (v parse_list_kind (list t)) opened
+    (aparse (parse_list p) a0 va0)
+    (fun va ->
+      aparse (parse_list p) a0 va `star`
+      list_iterator_strong p va0 a0 [] va
+    )
+    (k.parser_kind_subkind == Some ParserStrong)
+    (fun va -> va0.contents == va.contents)
+
+let list_iterator_begin
   (#opened: _)
   (#k: parser_kind)
   (#t: Type)
@@ -47,8 +119,27 @@ val list_iterator_begin
     )
     (k.parser_kind_subkind == Some ParserStrong)
     (fun va -> va0.contents == va.contents)
+= let va = list_iterator_strong_begin p a0 in
+  list_iterator_of_list_iterator_strong _ _ _ _ _;
+  va
 
-val list_iterator_end
+val list_iterator_strong_end
+  (#opened: _)
+  (#k: parser_kind)
+  (#t: Type)
+  (p: parser k t)
+  (#va0: v parse_list_kind (list t))
+  (#va: v parse_list_kind (list t))
+  (a0: byte_array)
+  (l: list t)
+  (a: byte_array)
+: STGhostT unit opened
+    (list_iterator_strong p va0 a0 l va `star`
+      aparse (parse_list p) a va)
+    (fun _ ->
+      aparse (parse_list p) a0 va0)
+
+let list_iterator_end
   (#opened: _)
   (#k: parser_kind)
   (#t: Type)
@@ -62,8 +153,32 @@ val list_iterator_end
       aparse (parse_list p) a va)
     (fun _ ->
       aparse (parse_list p) a0 va0)
+= let _ = list_iterator_strong_of_list_iterator _ _ _ _ in
+  list_iterator_strong_end _ _ _ _
 
-val list_iterator_append
+val list_iterator_strong_append
+  (#opened: _)
+  (#k: parser_kind)
+  (#t: Type)
+  (p: parser k t)
+  (#va0: v parse_list_kind (list t))
+  (#va: v parse_list_kind (list t))
+  (#va1: v parse_list_kind (list t))
+  (a0: byte_array)
+  (l: list t)
+  (a1: byte_array)
+  (va2: v parse_list_kind (list t))
+: STGhost unit opened
+    (list_iterator_strong p va0 a0 l va `star`
+      aparse (parse_list p) a1 va1)
+    (fun a ->
+      list_iterator_strong p va0 a0 (l `List.Tot.append` va1.contents) va2)
+    (AP.merge_into (array_of va1) (array_of va2) (array_of va) /\
+      va.contents == va1.contents `List.Tot.append` va2.contents
+    )
+    (fun _ -> True)
+
+let list_iterator_append
   (#opened: _)
   (#k: parser_kind)
   (#t: Type)
@@ -83,8 +198,34 @@ val list_iterator_append
       va.contents == va1.contents `List.Tot.append` va2.contents
     )
     (fun _ -> True)
+= let _ = list_iterator_strong_of_list_iterator _ _ _ _ in
+  list_iterator_strong_append _ _ _ _ _;
+  list_iterator_of_list_iterator_strong _ _ _ _ _
 
-val list_iterator_next
+val list_iterator_strong_next
+  (#opened: _)
+  (#k: parser_kind)
+  (#t: Type)
+  (p: parser k t)
+  (#va0: v parse_list_kind (list t))
+  (#va: v parse_list_kind (list t))
+  (#va1: v k t)
+  (a0: byte_array)
+  (l: list t)
+  (a1: byte_array)
+  (va2: v parse_list_kind (list t))
+: STGhost unit opened
+    (list_iterator_strong p va0 a0 l va `star`
+      aparse p a1 va1)
+    (fun a ->
+      list_iterator_strong p va0 a0 (l `List.Tot.append` [va1.contents]) va2)
+    (AP.merge_into (array_of va1) (array_of va2) (array_of va) /\
+      AP.length (array_of va1) > 0 /\
+      va.contents == va1.contents :: va2.contents
+    )
+    (fun _ -> True)
+
+let list_iterator_next
   (#opened: _)
   (#k: parser_kind)
   (#t: Type)
@@ -105,6 +246,9 @@ val list_iterator_next
       va.contents == va1.contents :: va2.contents
     )
     (fun _ -> True)
+= let _ = list_iterator_strong_of_list_iterator _ _ _ _ in
+  list_iterator_strong_next _ _ _ _ _;
+  list_iterator_of_list_iterator_strong _ _ _ _ _
 
 val list_slice
   (#k: parser_kind)
